\section{It$\mathrm{\^o}$'s Formulas}

%\begin{frame}
%  \frametitle{Differentiation and Integration of Stochastic Processes}
%
%  \begin{itemize}
%   \item Brownian motion is a continuous time stochastic process that is nowhere differentiable.\\
%  \item  How do we make sense of $\frac{dB}{dt}$?\\
%\end{itemize}
%
%\end{frame}

\begin{frame}
  \frametitle{Riemann-Stieltjes Integration of Stochastic Processes}
  \begin{itemize}
  \item $$\int_{a}^{b} f(x) d\alpha(x)=\lim_{n\to\infty}\sum_{i=1}^{n} f(x_i) (\alpha(x_i)-\alpha(x_{i-1}))$$\\
  \item  $$\int_{a}^{b} f(t) dB=\lim_{n\to\infty}\sum_{i=1}^{n} f(t_{i-1}) (B(t_i)-B(t_{i-1}))$$\\
  %\item  Form the Taylor expansion on $f(B(b))-f(B(a))$\\
  \end{itemize}
\end{frame}


\begin{frame}
  \frametitle{Left and Right Riemann-Stieltjes Sums}
  \begin{itemize}
  \item Left Riemann-Stieltjes sum $$L=\lim_{n\to\infty}\sum_{i=1}^{n} f(t_{i-1}) (B(t_i)-B(t_{i-1}))$$\\
  \item Right Riemann-Stieltjes sum $$R=\lim_{n\to\infty}\sum_{i=1}^{n} f(t_i) (B(t_i)-B(t_{i-1}))$$\\

  \end{itemize}
\end{frame}
  
\begin{frame}
  \frametitle{Left and Right Riemann-Stieltjes Sums}
  \begin{itemize}
      \item Considering $$\int_{a}^{b}{B(t)d(B(t))}$$\\
  \item The left solution $$L=\frac{1}{2}B^2(t)-\frac{t}{2}$$\\
  \item The right solution $$R=\frac{1}{2}B^2(t)+\frac{t}{2}$$\\
  \end{itemize}  
\end{frame}
  
\begin{frame}
  \frametitle{It$\mathrm{\^o}$'s Formula (First Formulation)}
  \begin{itemize}
  \item $\Delta B^2 \to \Delta t$\\
  \item  The Taylor expansion is
  \begin{eqnarray*}
    f(B(t_i))-f(B(t_{i-1}))&=&f'(B(t_{i-1}))(B(t_i)-B(t_{i-1}))+\\
    & &\frac{1}{2}f''(B(t_{i-1}))(B(t_i)-B(t_{i-1}))^2+\\
    %& &\frac{1}{3}f'''(B(t_{i-1}))(B(t_i)-B(t_{i-1}))^3+\\
    & &\mathrm{Higher Order Terms}\\
  \end{eqnarray*}
  %f(B(b))-f(B(a))&=&\sum_{i=1}^{n}(f'(B(t_{i-1}))(B(t_i)-B(t_{i-1}))+\\
  %& &\frac{1}{2}f''(B(t_{i-1}))(B(t_i)-B(t_{i-1}))^2+\\
  %& &\frac{1}{3}f'''(B(t_{i-1}))(B(t_i)-B(t_{i-1}))^3+\\
  %& &\mathrm{Higher Order Terms})\\
  \item Taking the sum of the telescoping series $$f(B(b))-f(B(a))=\sum_{i=1}^{n}(f(B(t_i))-f(B(t_{i-1})))$$\\
  \item It$\mathrm{\^o}$'s Formula (first version) $$f(B(b))-f(B(a))=\int_{a}^{b}{\frac{\partial f}{\partial B} dB}+\int_{a}^{b}{\frac{1}{2} \frac{\partial^2 f}{\partial B^2} dt} $$\\
  \end{itemize}
\end{frame}

\begin{frame}
  \frametitle{It$\mathrm{\^o}$'s Formula (Second and Third Formulation)}
  \begin{itemize}
  \item  It$\mathrm{\^o}$'s Formula (second version) $$f(b,B(b))-f(a,B(a))=\int_{a}^{b}{\frac{\partial f}{\partial B} dB}+\int_{a}^{b}{(\frac{\partial f}{\partial s}+\frac{1}{2}\frac{\partial ^2 f}{\partial B^2}) ds}$$\\
  \item  It$\mathrm{\^o}$'s Formula (third version): The Stochastic Chain Rule $$d\theta=\frac{\partial\theta}{\partial t}dt+\frac{\partial\theta}{\partial x}f dB+\frac{\partial\theta}{\partial x}g dt+\frac{1}{2}\frac{\partial^2\theta}{\partial x^2}f^2dt$$\\
  where $\theta$ is a function of t and x\\
  and f and g are functions of t and B\\
  and x satisfies $dx=fdt+gdB$
  \end{itemize}
  
\end{frame}

%\begin{frame}
%  \frametitle{Integration by Parts}
%  \begin{itemize}
%  \item $$\int_{a}^{b}{f(t)dB}=f(t)B(t)|_{a}^{b}-\int_{a}^{b}{B(t)df}$$
%  \end{itemize}

%\end{frame}





%%% Local Variables:
%%% mode: latex
%%% TeX-master: "Presentation1"
%%% End:

\
